move tests to their own files

barrier/heap_lang.v
@@ -405,30 +405,6 @@ Proof.
     try (destruct_conjs; eapply fill_not_value2; eassumption).
 Qed.
 
-(** Tests, making sure that stuff works. *)
-Module Tests.
-  Definition add := Op2 plus (Lit 21) (Lit 21).
-
-  Goal forall σ, prim_step add σ (Lit 42) σ None.
-  Proof.
-    apply Op2S.
-  Qed.
-
-  Definition rec := Rec (App (Var 1) (Var 0)). (* fix f x => f x *)
-  Definition rec_app := App rec (Lit 0).
-  Goal forall σ, prim_step rec_app σ rec_app σ None.
-  Proof.
-    move=>?. eapply BetaS. (* Honestly, I have no idea why this works. *)
-    reflexivity.
-  Qed.
-
-  Definition lam := Lam (Op2 plus (Var 0) (Lit 21)).
-  Goal forall σ, prim_step (App lam (Lit 21)) σ add σ None.
-  Proof.
-    move=>?. eapply BetaS. reflexivity.
-  Qed.
-End Tests.
-
 (** Instantiate the Iris language interface. This closes reduction under
     evaluation contexts.
     We could potentially make this a generic construction. *)
