barrier/parameter.v
@@ -2,4 +2,3 @@ Require Export barrier.heap_lang.
 Require Import iris.parameter.
 
 Definition Σ := IParamConst heap_lang unitRA.
-Print Assumptions Σ.
