barrier/tests.v
@@ -1,0 +1,30 @@
+(** This file is essentially a bunch of testcases. *)
+Require Import modures.base.
+Require Import barrier.lifting.
+
+Module LangTests.
+  Definition add := Op2 plus (Lit 21) (Lit 21).
+
+  Goal ∀ σ, prim_step add σ (Lit 42) σ None.
+  Proof.
+    apply Op2S.
+  Qed.
+
+  Definition rec := Rec (App (Var 1) (Var 0)). (* fix f x => f x *)
+  Definition rec_app := App rec (Lit 0).
+  Goal ∀ σ, prim_step rec_app σ rec_app σ None.
+  Proof.
+    move=>?. eapply BetaS. (* Honestly, I have no idea why this works. *)
+    reflexivity.
+  Qed.
+
+  Definition lam := Lam (Op2 plus (Var 0) (Lit 21)).
+  Goal ∀ σ, prim_step (App lam (Lit 21)) σ add σ None.
+  Proof.
+    move=>?. eapply BetaS. reflexivity.
+  Qed.
+End LangTests.
+
+Module ParamTests.
+  Print Assumptions Σ.
+End ParamTests.
