iris/tests.v
@@ -1,0 +1,6 @@
+(** This file tests a bunch of things. *)
+Require Import iris.model.
+
+Module ModelTest. (* Make sure we got the notations right. *)
+  Definition iResTest (Σ : iParam) (w : iWld Σ) (p : iPst Σ) (g : iGst Σ) : iRes Σ := Res w p g.
+End ModelTest.
